dafny/GeneratedCSD.dfy
@@ -8,12 +8,13 @@ module GeneratedCSD {
     requires lm.ValidTokensIdsLogits()
     requires parser.IsValidPrefix([])
     requires forall t: Token :: t in parser.ValidNextTokens([]) ==> t in lm.Tokens
-    requires "<<" in lm.Tokens && ">>" in lm.Tokens
+    requires LeftDelimiter in lm.Tokens && RightDelimiter in lm.Tokens
     ensures lm.ValidTokensIdsLogits()
     ensures |generated| <= maxSteps
     ensures remainingSteps >= 0 && remainingSteps <= maxSteps
   {
-    var helpers := new CSDHelpers();
+    var delim := new Delimiter(LeftDelimiter, RightDelimiter);
+    var helpers := new CSDHelpers(lm, parser, delim);
     var stepsLeft := maxSteps;
     // QWEN_INSERT_STRATEGY_HERE
     remainingSteps := stepsLeft;
